Create module interfaces for Interop_s and GenericInterop2

vale/code/arch/x64/interop/GenericInterop2.fsti
@@ -1,1 +1,288 @@
 module GenericInterop2
+
+open LowStar.Buffer
+module B = LowStar.Buffer
+module BV = LowStar.BufferView
+open LowStar.Modifies
+module M = LowStar.Modifies
+open LowStar.ModifiesPat
+open FStar.HyperStack.ST
+module HS = FStar.HyperStack
+open Interop
+open Words_s
+open Types_s
+open X64.Machine_s
+open X64.Memory_s
+open X64.Vale.State
+open X64.Vale.Decls
+open BufferViewHelpers
+open Interop_assumptions
+open X64.Vale.StateLemmas
+open X64.Vale.Lemmas
+module TS = X64.Taint_Semantics_s
+module ME = X64.Memory_s
+module BS = X64.Bytes_Semantics_s
+module IS = X64.Interop_s
+open X64.Interop_s
+
+let initial_vale_state_t (dom:list vale_type) (acc:list b8) =
+  initial_state_t dom acc va_state
+
+val create_initial_vale_state_core
+       (acc:list b8)
+       (regs:registers)
+       (xmms:xmms_t)
+       (taint:taint_map)
+       (h0:HS.mem)
+       (stack:b8{mem_roots_p h0 (stack::acc)})
+  : GTot va_state
+
+val core_create_lemma
+       (acc:list b8)
+       (regs:registers)
+       (xmms:xmms_t)
+       (taint:taint_map)
+       (h0:HS.mem)
+       (stack:b8{mem_roots_p h0 (stack::acc)})
+  : Lemma
+      (ensures (fst (create_initial_trusted_state_core acc regs xmms taint h0 stack) ==
+                state_to_S (create_initial_vale_state_core acc regs xmms taint h0 stack)))
+
+let create_vale_initial_state_t (dom:list vale_type)
+                                (acc:list b8)
+    = n_dep_arrow
+          dom
+          (initial_vale_state_t dom acc)
+
+
+let elim_down_1 (hd:vale_type)
+                (acc:list b8)
+                (down:create_vale_initial_state_t [hd] acc)
+                (x:vale_type_as_type hd)
+    : h0:HS.mem -> stack:b8{mem_roots_p h0 (stack::maybe_cons_buffer hd x acc)} -> GTot va_state =
+    down x
+
+let elim_down_nil (acc:list b8)
+                  (down:create_vale_initial_state_t [] acc)
+    : h0:HS.mem -> stack:b8{mem_roots_p h0 (stack::acc)} -> GTot va_state =
+    down
+
+let elim_down_cons (hd:vale_type)
+                   (tl:list vale_type)
+                   (acc:list b8)
+                   (down:create_vale_initial_state_t (hd::tl) acc)
+                   (x:vale_type_as_type hd)
+    : create_vale_initial_state_t tl (maybe_cons_buffer hd x acc) =
+    elim_dep_arrow_cons hd tl down x
+
+//////////////////////////////////////////////////////////////////////////////////////////
+//vale_sig pre post: a template for a top-level signature provided by a vale function
+//////////////////////////////////////////////////////////////////////////////////////////
+
+let vale_pre_tl (dom:list vale_type) =
+    n_arrow dom (va_state -> stack_buffer -> prop)
+
+let vale_pre (dom:list vale_type) =
+    code:va_code ->
+    win:bool ->
+    vale_pre_tl dom
+
+let vale_post_tl (dom:list vale_type) =
+    n_arrow dom
+            (s0:va_state -> sb:stack_buffer -> s1:va_state -> f:va_fuel -> prop)
+
+let vale_post (dom:list vale_type) =
+    code:va_code ->
+    win:bool ->
+    vale_post_tl dom
+
+let vale_save_reg (r:reg) (s0 s1:va_state) =
+  eval_reg r s0 == eval_reg r s1
+
+let vale_save_xmm (r:xmm) (s0 s1:va_state) =
+  eval_xmm r s0 == eval_xmm r s1
+
+let vale_calling_conventions (win:bool) (s0 s1:va_state) =
+  vale_save_reg Rbx s0 s1 /\
+  (win ==> vale_save_reg Rsi s0 s1) /\
+  (win ==> vale_save_reg Rdi s0 s1) /\
+  vale_save_reg Rbp s0 s1 /\
+  (win ==> vale_save_reg Rsp s0 s1) /\ // TODO: also needed for !win
+  vale_save_reg R12 s0 s1 /\
+  vale_save_reg R13 s0 s1 /\
+  vale_save_reg R14 s0 s1 /\
+  vale_save_reg R15 s0 s1 /\
+  (win ==>
+    vale_save_xmm 6 s0 s1 /\
+    vale_save_xmm 7 s0 s1 /\
+    vale_save_xmm 8 s0 s1 /\
+    vale_save_xmm 9 s0 s1 /\
+    vale_save_xmm 10 s0 s1 /\
+    vale_save_xmm 11 s0 s1 /\
+    vale_save_xmm 12 s0 s1 /\
+    vale_save_xmm 13 s0 s1 /\
+    vale_save_xmm 14 s0 s1 /\
+    vale_save_xmm 15 s0 s1
+  ) /\
+  s1.ok
+
+let rec vale_sig_tl (#dom:list vale_type)
+                    (code:va_code)
+                    (win:bool)
+                    (pre:vale_pre_tl dom)
+                    (post:vale_post_tl dom)
+  : Type =
+    match dom with
+    | [] ->
+      va_s0:va_state ->
+      stack_b:stack_buffer ->
+      Ghost (va_state & va_fuel)
+            (requires (elim_nil pre va_s0 stack_b))
+            (ensures (fun (va_s1, f) ->
+                       X64.Vale.Decls.eval_code code va_s0 f va_s1 /\
+                       vale_calling_conventions win va_s0 va_s1 /\
+                       elim_nil post va_s0 stack_b va_s1 f))
+
+    | hd::tl ->
+      x:vale_type_as_type hd ->
+      vale_sig_tl #tl code win (elim_1 pre x) (elim_1 post x)
+
+let elim_vale_sig_cons #code
+                       (hd:vale_type)
+                       (tl:list vale_type)
+                       (pre:vale_pre_tl (hd::tl))
+                       (post:vale_post_tl (hd::tl))
+                       (v:vale_sig_tl code win pre post)
+    : x:vale_type_as_type hd
+    -> vale_sig_tl code win (elim_1 pre x) (elim_1 post x)
+    = v
+
+let vale_sig (#dom:list vale_type)
+             (pre:vale_pre dom)
+             (post:vale_post dom)
+  : Type =
+    code:va_code ->
+    win:bool ->
+    vale_sig_tl code win (pre code win)
+                     (post code win)
+
+//////////////////////////////////////////////////////////////////////////////////////////
+//lowstar_sig pre post:
+//    Interepreting a vale pre/post as a Low* function type
+//////////////////////////////////////////////////////////////////////////////////////////
+
+val as_lowstar_sig_tl_req (code:va_code)
+                          (acc:list b8)
+                          (down:create_vale_initial_state_t [] acc)
+                          (pre: vale_pre_tl [])
+                          (post: vale_post_tl [])
+                          (h0 : HS.mem) : Type0
+
+val as_lowstar_sig_tl_ens (code:va_code)
+                          (acc:list b8)
+                          (down:create_vale_initial_state_t [] acc)
+                          (pre: vale_pre_tl [])
+                          (post: vale_post_tl [])
+                          (h0 : HS.mem)
+                          (_ : unit)
+                          (h1 : HS.mem) : Type0
+
+let rec as_lowstar_sig_tl (#dom:list vale_type)
+                          (code:va_code)
+                          (acc:list b8)
+                          (down:create_vale_initial_state_t dom acc)
+                          (pre: vale_pre_tl dom)
+                          (post: vale_post_tl dom)
+    : Type =
+    match dom with
+    | [] ->
+      unit ->
+      Stack unit
+        (requires as_lowstar_sig_tl_req code acc down pre post)
+        (ensures as_lowstar_sig_tl_ens code acc down pre post)
+    | hd::tl ->
+      x:vale_type_as_type hd ->
+      as_lowstar_sig_tl
+        #tl
+        code
+        (maybe_cons_buffer hd x acc)
+        (elim_down_cons hd tl acc down x)
+        (elim_1 pre x)
+        (elim_1 post x)
+
+let create_vale_initial_state
+      (is_win:bool)
+      (dom:list vale_type{List.length dom < max_arity is_win})
+    : create_vale_initial_state_t dom []
+    = create_initial_state_aux
+          dom
+          is_win
+          0
+          init_regs
+          init_xmms
+          []
+          init_taint
+          create_initial_vale_state_core
+
+let as_lowstar_sig  (c:va_code) (dom:list vale_type{List.length dom < max_arity win})
+                    (pre: vale_pre dom)
+                    (post: vale_post dom) =
+    unit ->
+    as_lowstar_sig_tl
+      #dom
+      c
+      []
+      (create_vale_initial_state win dom)
+      (pre c win)
+      (post c win)
+
+////////////////////////////////////////////////////////////////////////////////
+
+let elim_vale_sig_nil  #code #win
+                       (pre:vale_pre_tl [])
+                       (post:vale_post_tl [])
+                       (v:vale_sig_tl code win pre post)
+    : va_s0:va_state ->
+      stack_b:stack_buffer ->
+      Ghost (va_state & va_fuel)
+            (requires (elim_nil pre va_s0 stack_b))
+            (ensures (fun (va_s1, f) -> elim_nil post va_s0 stack_b va_s1 f))
+    = v
+
+let elim_trusted_lowstar_sig_nil
+      #code
+      (acc:list b8)
+      (down:create_trusted_initial_state_t [] acc)
+      (v:IS.as_lowstar_sig_tl code [] acc down)
+    : h0:HS.mem ->
+      predict:prediction code acc down h0 ->
+      Stack (as_lowstar_sig_ret acc)
+        (requires (fun h0' -> h0 == h0' /\ mem_roots_p h0 acc /\ True))
+        (ensures (fun h0 (As_lowstar_sig_ret push_h0 alloc_push_h0 b fuel final_mem) h1 ->
+          IS.as_lowstar_sig_post code acc down h0 predict push_h0 alloc_push_h0 b fuel final_mem h1))
+    = v
+
+let elim_trusted_lowstar_sig_cons
+      #code
+      (hd:vale_type)
+      (tl:list vale_type)
+      (acc:list b8)
+      (down:create_trusted_initial_state_t (hd::tl) acc)
+      (v:IS.as_lowstar_sig_tl code (hd::tl) acc down)
+    : x:vale_type_as_type hd ->
+      IS.as_lowstar_sig_tl
+        code
+        tl
+        (maybe_cons_buffer hd x acc)
+        (IS.elim_down_cons hd tl acc down x)
+    = v
+
+val lower_code (c:va_code) : code
+
+val wrap (code:va_code) (dom:list vale_type{List.length dom < max_arity win})
+         (pre:vale_pre dom)
+         (post:vale_post dom)
+         (v:vale_sig pre post)
+         (t_low:IS.as_lowstar_sig (lower_code code) dom)
+  : as_lowstar_sig code dom pre post
+
