vale/specs/hardware/X64.Interop_s.fst
@@ -28,273 +28,13 @@ friend X64.Memory
 //friend X64.Vale.Decls
 //friend X64.Vale.StateLemmas
 
-unfold let code = TS.tainted_code
-
-////////////////////////////////////////////////////////////////////////////////
-// Vale-specific types supported by the interop layer
-//   Some integer types
-//   And arrays thereof
-////////////////////////////////////////////////////////////////////////////////
-
-type vale_type =
-  | VT_Base of X64.Memory_s.base_typ
-  | VT_Buffer of X64.Memory_s.base_typ
-
-#set-options "--initial_ifuel 1"
-let base_type_as_type : X64.Memory_s.base_typ -> Type =
-  function
-  | TUInt8 -> UInt8.t
-  | TUInt16 -> UInt16.t
-  | TUInt32 -> UInt32.t
-  | TUInt64 -> UInt64.t
-  | TUInt128 -> False
-
-let vale_type_as_type : vale_type -> Type =
-  function
-  | VT_Base bt -> base_type_as_type bt
-  | VT_Buffer bt -> X64.Memory_s.buffer (TBase bt)
-
-
-////////////////////////////////////////////////////////////////////////////////
-// as_l/r_tuple: Interpreting a list of vale types as
-//               a left- or right-nested pair
-////////////////////////////////////////////////////////////////////////////////
-let rec as_right_tuple (dom:list vale_type{Cons? dom}) =
-  match dom with
-  | [x] -> vale_type_as_type x
-  | hd::tl -> vale_type_as_type hd & as_right_tuple tl
-
-let rec as_left_tuple (acc:Type) (dom:list vale_type)
-  : Tot Type (decreases dom) =
-  match dom with
-  | [] -> acc
-  | hd::tl -> as_left_tuple (acc & vale_type_as_type hd) tl
-
-////////////////////////////////////////////////////////////////////////////////
-// n_arrow: Arrows with a generic number of vale types as the domain
-//          and a result type `codom` that does not depend on the domain
-////////////////////////////////////////////////////////////////////////////////
-[@unifier_hint_injective]
-let rec n_arrow (dom:list vale_type) (codom:Type) =
-  match dom with
-  | [] -> codom
-  | hd::tl -> vale_type_as_type hd -> n_arrow tl codom
-
-[@unifier_hint_injective]
-let arr (dom:Type) (codom:Type) = dom -> codom
-
-let elim_1 (#dom:list vale_type{Cons? dom})
-           (#r:Type)
-           (f:n_arrow dom r)
-    : vale_type_as_type (Cons?.hd dom) -> n_arrow (Cons?.tl dom) r =
-    f
-
-let elim_nil (#dom:list vale_type{Nil? dom})
-           (#r:Type)
-           (f:n_arrow dom r)
-    : r =
-    f
-
-let intro_n_arrow_nil (a:Type) (x:a)
-  : n_arrow [] a
-  = x
-
-let intro_n_arrow_cons (hd:vale_type) (b:Type) (tl:list vale_type)
-                       (x:vale_type_as_type hd -> n_arrow tl b)
-  : n_arrow (hd::tl) b
-  = x
-
-////////////////////////////////////////////////////////////////////////////////
-// n_dep_arrow: Arrows with a generic number of vale types as the domain
-//              and a result type codom that depends on the domain
-////////////////////////////////////////////////////////////////////////////////
-[@unifier_hint_injective]
-let rec n_dep_arrow (dom:list vale_type) (codom: n_arrow dom Type) =
-  match dom with
-  | [] -> codom
-  | hd::tl -> x:vale_type_as_type hd -> n_dep_arrow tl (elim_1 codom x)
-
-let intro_dep_arrow_nil (b:Type)
-                        (f:b)
-  : n_dep_arrow [] b
-  = f
-
-let intro_dep_arrow_1 (a:vale_type)
-                      (b:n_arrow [a] Type)
-                      (f:(x:vale_type_as_type a -> elim_1 b x))
-  : n_dep_arrow [a] b
-  = f
-
-let intro_dep_arrow_cons (hd:vale_type)
-                         (tl:list vale_type)
-                         (b: n_arrow (hd::tl) Type)
-                         (f: (x:vale_type_as_type hd -> n_dep_arrow tl (elim_1 b x)))
-  : n_dep_arrow (hd::tl) b
-  = f
-
-let elim_dep_arrow_nil (#codom:n_arrow [] Type)
-                       (f:n_dep_arrow [] codom)
-    : elim_nil codom
-   = f
-
-let elim_dep_arrow_cons (hd:vale_type)
-                        (tl:list vale_type)
-                        (#codom:n_arrow (hd::tl) Type)
-                        (f:n_dep_arrow (hd::tl) codom)
-    : x:vale_type_as_type hd ->
-      n_dep_arrow tl (elim_1 codom x)
-   = f
-
-//Just a small test function to see how these coercions work
-let test : n_dep_arrow [VT_Base TUInt8] (fun (x:UInt8.t) -> y:UInt8.t{x == y}) =
-  fun (x:UInt8.t) -> intro_dep_arrow_nil (y:UInt8.t{x == y}) x
-
-////////////////////////////////////////////////////////////////////////////////
-// Creating initial states
-// The punchline of this section is the `create_both_initial_states`,
-// an arity generic function that builds a trusted state `t:TS.state`
-// and a vale state `v:va_state` with a proof that `t == state_to_S v`
-////////////////////////////////////////////////////////////////////////////////
-
-let maybe_cons_buffer (a:vale_type) (x:vale_type_as_type a) (acc:list b8) : list b8 =
-  if VT_Buffer? a then x::acc else acc
-
-let mem_roots_p (h0:HS.mem) (roots:list b8) =
-  Interop.list_disjoint_or_eq roots /\
-  Interop.list_live h0 roots
-
-let mem_roots (roots:list b8) =
-    h0:HS.mem{ mem_roots_p h0 roots }
-
-let rec initial_state_t
-              (dom:list vale_type)
-              (acc:list b8)
-              (codom:Type)
-  : n_arrow dom Type =
-    match dom with
-    | [] ->
-      (h0:HS.mem ->
-       stack:b8{mem_roots_p h0 (stack::acc)} ->
-       GTot codom)
-    | hd::tl ->
-      fun (x:vale_type_as_type hd) ->
-         initial_state_t tl (maybe_cons_buffer hd x acc) codom
-
-// Some identity coercions that serve as proof hints
-// to introduce generic arrow types
-let fold_initial_state_t
-  (#hd:vale_type) (#tl:list vale_type)
-  (#x:vale_type_as_type hd) (#acc:list b8) (#codom:Type)
-  (res:n_dep_arrow tl (initial_state_t tl (maybe_cons_buffer hd x acc) codom))
-  : n_dep_arrow tl (elim_1 (initial_state_t (hd::tl) acc codom) x)
-  = res
-
-let initial_trusted_state_t (dom:list vale_type) (acc:list b8) =
-  initial_state_t dom acc (TS.traceState & mem)
-
-////////////////////////////////////////////////////////////////////////////////
-//The calling convention w.r.t the register mapping
-////////////////////////////////////////////////////////////////////////////////
-let max_arity (is_win:bool) = if is_win then 4 else 6
-
-let register_of_arg_i (is_win:bool) (i:nat{i < max_arity is_win}) : reg =
-  if is_win then
-    match i with
-    | 0 -> Rcx
-    | 1 -> Rdx
-    | 2 -> R8
-    | 3 -> R9
-  else
-    match i with
-    | 0 -> Rdi
-    | 1 -> Rsi
-    | 2 -> Rdx
-    | 3 -> Rcx
-    | 4 -> R8
-    | 5 -> R9
-
-//A partial inverse of the above function
-let arg_of_register (is_win:bool) (r:reg)
-  : option (i:nat{i < max_arity is_win /\ register_of_arg_i is_win i = r})
-  = if is_win then
-       match r with
-       | Rcx -> Some 0
-       | Rdx -> Some 1
-       | R8 -> Some 2
-       | R9 -> Some 3
-       | _ -> None
-    else
-       match r with
-       | Rdi -> Some 0
-       | Rsi -> Some 1
-       | Rdx -> Some 2
-       | Rcx -> Some 3
-       | R8 -> Some 4
-       | R9 -> Some 5
-       | _ -> None
-
-let registers = reg -> nat64
-
-let update_regs (#a:vale_type)
-                (x:vale_type_as_type a)
-                (is_win:bool)
-                (i:nat{i < max_arity is_win})
-                (regs:registers)
-  : registers
-  =
-    let value : nat64 =
-      match a with
-      | VT_Base TUInt8 ->
-        UInt8.v x
-      | VT_Base TUInt16 ->
-        UInt16.v x
-      | VT_Base TUInt32 ->
-        UInt32.v x
-      | VT_Base TUInt64 ->
-        UInt64.v x
-      | VT_Buffer _ ->
-        addrs x
-    in
-    fun (r:reg) ->
-      match arg_of_register is_win r with
-      | Some j ->
-        if i = j then value
-        else regs r
-      | _ -> regs r
-
-let xmms_t = xmm -> quad32
-
-let taint_map = b8 -> GTot taint
-
-let update_taint_map (#a:vale_type)
-                     (x:vale_type_as_type a)
-                     (taint:taint_map) =
-    match a with
-    | VT_Buffer _ ->
-      fun (y:b8) ->
-        if StrongExcludedMiddle.strong_excluded_middle ((x <: b8) == y) then
-          Secret
-        else taint y
-    | _ -> taint
-
-let regs_with_stack (regs:registers) (stack_b:b8) : registers =
-    fun r ->
-      if r = Rsp then
-        addrs stack_b
-      else regs r
+let to_b8 #bt m = m
 
 // Splitting the construction of the initial state into two functions
 // one that creates the initial trusted state (i.e., part of our TCB)
 // and another that just creates the vale state, a view upon the trusted one
-let create_initial_trusted_state_core
-       (acc:list b8)
-       (regs:registers)
-       (xmms:xmms_t)
-       (taint:taint_map)
-       (h0:HS.mem)
-       (stack:b8{mem_roots_p h0 (stack::acc)})
-  : GTot (TS.traceState & mem)
-  = let acc = stack::acc in
+let create_initial_trusted_state_core acc regs xmms taint h0 stack =
+    let acc = stack::acc in
     let (mem:mem) = {
       addrs = addrs;
       ptrs = acc;
@@ -316,164 +56,33 @@ let create_initial_trusted_state_core
     },
     mem
 
-//The type of an arity-generic function that produces a pair
-//of related trusted and vale states
-let trusted_initial_state_t (dom:list vale_type) (acc:list b8) =
-  initial_state_t dom acc (TS.traceState & mem)
+let prediction_pre c acc down h0 s0 push_h0 alloc_push_h0 b =
+  HS.fresh_frame h0 push_h0 /\
+  M.modifies loc_none push_h0 alloc_push_h0 /\
+  HS.get_tip push_h0 == HS.get_tip alloc_push_h0 /\
+  B.frameOf b == HS.get_tip alloc_push_h0 /\
+  B.live alloc_push_h0 b /\
+  s0 == fst (elim_down_nil acc down alloc_push_h0 b)
 
-//This function folds over the `dom:list vale_type`
-//and builds an arity-generic dependent function that constructs
-//the initial states
-//It's maybe more generic than it needs to be, since it is now applied only
-//once, i.e., with f = create_both_initial_states
-let rec create_initial_state_aux
-        #codom
-        (dom:list vale_type)
-        (is_win:bool)
-        (i:nat{i + List.length dom < max_arity is_win})
-        (regs:registers)
-        (xmms:xmms_t)
-        (acc:list b8)
-        (taint:taint_map)
-        (f: (acc:list b8 -> registers -> xmms_t -> taint_map -> h:HS.mem -> stack:b8{mem_roots_p h (stack::acc)} -> GTot codom))
-      : n_dep_arrow
-        dom
-        (initial_state_t dom acc codom) =
-        match dom with
-        | [] ->
-          //no more args; build the state from a HS.mem
-          intro_dep_arrow_nil
-              (initial_state_t [] acc codom)
-              (f acc regs xmms taint)
+let prediction_post c acc down h0 s0 push_h0 alloc_push_h0 b (fuel, final_mem) =
+  Some? (TS.taint_eval_code c fuel s0) /\ (
+    let sN = Some?.v (TS.taint_eval_code c fuel s0) in
+    Interop.down_mem final_mem.hs final_mem.addrs final_mem.ptrs == sN.TS.state.BS.mem /\
+    Interop_assumptions.calling_conventions win s0 sN
+//    save_reg Rbx s0 sN /\
+//    save_reg Rsi s0 sN /\
+//    save_reg Rdi s0 sN /\
+//    save_reg Rbp s0 sN /\
+//    save_reg Rsp s0 sN /\
+//    save_reg R12 s0 sN /\
+//    save_reg R13 s0 sN /\
+//    save_reg R14 s0 sN /\
+//    save_reg R15 s0 sN /\
+//    // TODO: callee-save for xmms
+//    sN.TS.state.BS.ok
+  )
 
-        | hd::tl ->
-          //put the next arg hd in the ith register
-          //update the taint map
-          //maybe add the next arg to the list of buffers
-          //recur
-          intro_dep_arrow_cons
-              hd
-              tl
-              (initial_state_t dom acc codom)
-              (fun (x:vale_type_as_type hd) ->
-                fold_initial_state_t
-                  (create_initial_state_aux
-                    tl
-                    is_win
-                    (i + 1)
-                    (update_regs x is_win i regs)
-                    xmms
-                    (maybe_cons_buffer hd x acc)
-                    (update_taint_map x taint)
-                    f))
-
-let init_taint : taint_map = fun r -> Public
-
-let create_trusted_initial_state_t (dom:list vale_type)
-                                (acc:list b8)
-    = n_dep_arrow
-          dom
-          (initial_trusted_state_t dom acc)
-
-let create_trusted_initial_state
-      (is_win:bool)
-      (dom:list vale_type{List.length dom < max_arity is_win})
-    : create_trusted_initial_state_t dom []
-    = create_initial_state_aux
-          dom
-          is_win
-          0
-          init_regs
-          init_xmms
-          []
-          init_taint
-          create_initial_trusted_state_core
-
-let stack_buffer = buffer (TBase TUInt64)
-
-//////////////////////////////////////////////////////////////////////////////////////////
-//lowstar_sig:
-//    Interepreting an assembly language type as a Low* function type
-//////////////////////////////////////////////////////////////////////////////////////////
-
-let elim_down_1 (hd:vale_type)
-                (acc:list b8)
-                (down:create_trusted_initial_state_t [hd] acc)
-                (x:vale_type_as_type hd)
-    : h0:HS.mem -> stack:b8{mem_roots_p h0 (stack::maybe_cons_buffer hd x acc)} -> GTot (TS.traceState & mem) =
-    down x
-
-let elim_down_nil (acc:list b8)
-                  (down:create_trusted_initial_state_t [] acc)
-    : h0:HS.mem -> stack:b8{mem_roots_p h0 (stack::acc)} -> GTot (TS.traceState & mem) =
-    down
-
-let save_reg (r:reg) (s0 sN:TS.traceState) =
-  BS.eval_reg r s0.TS.state == BS.eval_reg r sN.TS.state
-
-let elim_down_cons (hd:vale_type)
-                   (tl:list vale_type)
-                   (acc:list b8)
-                   (down:create_trusted_initial_state_t (hd::tl) acc)
-                   (x:vale_type_as_type hd)
-    : create_trusted_initial_state_t tl (maybe_cons_buffer hd x acc) =
-    elim_dep_arrow_cons hd tl down x
-
-// (stack_bytes:nat)
-// stack_b:b8 ->
-let prediction (c:code) (acc:list b8) (down:create_trusted_initial_state_t [] acc) (h0:HS.mem) =
-  s0:TS.traceState ->
-  push_h0:mem_roots acc ->
-  alloc_push_h0:mem_roots acc ->
-  b:stack_buffer{mem_roots_p alloc_push_h0 (b::acc)} ->
-  Ghost (nat & mem)
-    (requires
-      HS.fresh_frame h0 push_h0 /\
-      M.modifies loc_none push_h0 alloc_push_h0 /\
-      HS.get_tip push_h0 == HS.get_tip alloc_push_h0 /\
-      B.frameOf b == HS.get_tip alloc_push_h0 /\
-      B.live alloc_push_h0 b /\
-      s0 == fst (elim_down_nil acc down alloc_push_h0 b)
-    )
-    (ensures fun (fuel, final_mem) ->
-      Some? (TS.taint_eval_code c fuel s0) /\ (
-        let sN = Some?.v (TS.taint_eval_code c fuel s0) in
-        Interop.down_mem final_mem.hs final_mem.addrs final_mem.ptrs == sN.TS.state.BS.mem /\
-        save_reg Rbx s0 sN /\
-        save_reg Rsi s0 sN /\
-        save_reg Rdi s0 sN /\
-        save_reg Rbp s0 sN /\
-        save_reg Rsp s0 sN /\
-        save_reg R12 s0 sN /\
-        save_reg R13 s0 sN /\
-        save_reg R14 s0 sN /\
-        save_reg R15 s0 sN /\
-        // TODO: callee-save for xmms
-        sN.TS.state.BS.ok
-      )
-    )
-
-noeq type as_lowstar_sig_ret (acc:list b8) =
-  | As_lowstar_sig_ret :
-      push_h0:mem_roots acc ->
-      alloc_push_h0:mem_roots acc ->
-      b:stack_buffer{mem_roots_p alloc_push_h0 (b::acc)} ->
-      fuel:nat ->
-      final_mem:mem ->
-      as_lowstar_sig_ret acc
-
-let as_lowstar_sig_post
-    (c:code)
-    (acc:list b8)
-    (down:create_trusted_initial_state_t [] acc)
-    (h0:HS.mem)
-    (predict:prediction c acc down h0)
-    (push_h0:mem_roots acc)
-    (alloc_push_h0:mem_roots acc)
-    (b:stack_buffer{mem_roots_p alloc_push_h0 (b::acc)})
-    (fuel:nat)
-    (final_mem:mem)
-    (h1:HS.mem) =
+let as_lowstar_sig_post c acc down h0 predict push_h0 alloc_push_h0 b fuel final_mem h1 =
   let s0 = fst (elim_down_nil acc down alloc_push_h0 b) in
   HS.fresh_frame h0 push_h0 /\
   M.modifies loc_none push_h0 alloc_push_h0 /\
@@ -483,38 +92,6 @@ let as_lowstar_sig_post
   (fuel, final_mem) == predict s0 push_h0 alloc_push_h0 b /\
   HS.poppable final_mem.hs /\
   h1 == HS.pop (final_mem.hs)
-
-let rec as_lowstar_sig_tl
-    (c:code)
-    (dom:list vale_type)
-    (acc:list b8)
-    (down:create_trusted_initial_state_t dom acc)
-    : Type =
-    match dom with
-    | [] ->
-      h0:HS.mem ->
-      predict:prediction c acc down h0 ->
-      Stack (as_lowstar_sig_ret acc)
-        (requires (fun h0' -> h0 == h0' /\ mem_roots_p h0 acc))
-        (ensures fun h0 (As_lowstar_sig_ret push_h0 alloc_push_h0 b fuel final_mem) h1 ->
-          as_lowstar_sig_post c acc down h0 predict push_h0 alloc_push_h0 b fuel final_mem h1
-        )
-    | hd::tl ->
-      x:vale_type_as_type hd ->
-      as_lowstar_sig_tl
-        c
-        tl
-        (maybe_cons_buffer hd x acc)
-        (elim_down_cons hd tl acc down x)
-
-let as_lowstar_sig (c:code) (dom:list vale_type{List.length dom < max_arity win}) =
-    as_lowstar_sig_tl
-      c
-      dom
-      []
-      (create_trusted_initial_state win dom)
-
-////////////////////////////////////////////////////////////////////////////////
 
 let rec wrap_tl
          (c:code)
@@ -583,67 +160,5 @@ let rec wrap_tl
         f
 
 
-let wrap (c:code) (dom:list vale_type{List.length dom < max_arity win})
-  : as_lowstar_sig c dom =
-     wrap_tl c dom [] (create_trusted_initial_state win dom)
-
-(*
-////////////////////////////////////////////////////////////////////////////////
-//test
-////////////////////////////////////////////////////////////////////////////////
-open Vale_memcpy
-friend X64.Vale.Decls
-
-let c : code = va_code_memcpy true
-
-unfold
-let dom : l:list vale_type{List.Tot.length l < max_arity win} =
-  let d = [VT_Buffer TUInt64; VT_Buffer TUInt64;] in
-  assert_norm (List.Tot.length d < max_arity win);
-  d
-
-let memcpy_raw
-    : as_lowstar_sig c dom
-    = wrap c dom
-
-unfold let normal_steps : list string =
-  [
-    `%as_lowstar_sig;
-    `%as_lowstar_sig_tl;
-    `%vale_type_as_type;
-    `%VT_Buffer?;
-    `%maybe_cons_buffer;
-    `%elim_down_cons;
-    `%create_trusted_initial_state;
-//    `%create_initial_state_aux;
-//    `%elim_dep_arrow_nil;
-//    `%elim_dep_arrow_cons;
-  ]
-
-unfold let normal (#a:Type) (x:a) : a = norm [iota; zeta; simplify; primops; delta_only normal_steps] x
-//unfold let normal (#a:Type) (x:a) : a = norm [delta_only normal_steps] x
-
-let force (#a:Type) (x:a) : normal a = x
-
-#reset-options "--debug X64.Interop_s --debug_level print_normalized_terms --use_two_phase_tc false"
-//let elim_lowstar_sig (dom:list vale_type{List.length dom < max_arity win})
-//                     (f:as_lowstar_sig c dom)
-//    : (assume False; normal (as_lowstar_sig c dom))
-//    =
-//admit ()
-//    assume False;
-//    force #(as_lowstar_sig c dom) f
-
-val memcpy: dst:buffer64 -> src:buffer64 -> Stack unit
-        (requires (fun h -> True))
-        (ensures (fun h0 _ h1 -> True))
-let memcpy dst src =
-//  let f:normal (as_lowstar_sig c dom) = elim_lowstar_sig dom memcpy_raw in
-//  let f:normal (as_lowstar_sig c dom) = force #(as_lowstar_sig c dom) memcpy_raw in
-  let f1:normal (as_lowstar_sig c dom) = memcpy_raw in
-  let f2 = f1 dst src in
-  let h0 = get () in
-  let f3 = f2 h0 in
-//  f dst src ()
-()
-*)
+let wrap c dom =
+  wrap_tl c dom [] (create_trusted_initial_state win dom)
